MonadTrans Spec

MonadTrans.v
@@ -6,7 +6,7 @@ Require Export TypeClassLib.Monad.
 Class MonadTrans
       (T : (Type -> Type) -> Type -> Type) :=
   { (** Monadic Substructure *)
-    Trans_Monad :> forall {M : Type -> Type} `{Monad M}, Monad (T M);
+    Trans_Monad :> forall (M : Type -> Type) `{Monad M}, Monad (T M);
     lift : forall {M : Type -> Type} `{Monad M}
              {A : Type}, M A -> T M A;
     (** Lift with pure is idempotent. *)
@@ -17,3 +17,34 @@ Class MonadTrans
                   {A B : Type} (m : M A) (f : A -> M B),
         lift (bind m f) = bind (lift m) (lift ∘ f); }.
 (**[]*)
+
+(** Specification. *)
+Module Type MonadTransSpec.
+  Parameter T : (Type -> Type) -> Type -> Type.
+
+  Parameter TMonad : forall (M : Type -> Type) `{Monad M}, Monad (T M).
+
+  Parameter lift : forall {M : Type -> Type} `{Monad M}
+                     {A : Type}, M A -> T M A.
+  (**[]*)
+
+  Parameter lift_pure : forall {M : Type -> Type} `{Monad M} {A : Type},
+      @lift M _ A ∘ (@pure M _ A) =
+      @pure (T M) (@Monad_Applicative (T M) (TMonad M)) A.
+  (**[]*)
+
+  Parameter lift_bind : forall {M : Type -> Type} `{Monad M}
+                          {A B : Type} (m : M A) (f : A -> M B),
+      lift (bind m f) = @bind (T M) (TMonad M) _ _ (lift m) (lift ∘ f).
+  (**[]*)
+End MonadTransSpec.
+
+Module MonadTransFactory (MS : MonadTransSpec).
+  Include MS.
+
+  Instance MonadTransInstance : MonadTrans MS.T :=
+    { lift := @MS.lift;
+      lift_pure := @MS.lift_pure;
+      lift_bind := @MS.lift_bind }.
+  (**[]*)
+End MonadTransFactory.
